data_structure/spatial_graph_VST.v
@@ -1,4 +1,5 @@
-Require Import RamifyCoq.data_structure.spatial_graph2.
+Require Import RamifyCoq.data_structure.general_spatial_graph.
+Require Import RamifyCoq.data_structure.spatial_graph_mark.
 Require Import RamifyCoq.msl_ext.abs_addr.
 Require Import RamifyCoq.msl_ext.seplog.
 Require Import VST.veric.SeparationLogic.
@@ -7,21 +8,47 @@ Require Import RamifyCoq.msl_ext.alg_seplog.
 Require Import RamifyCoq.sample_mark.env_mark.
 Require Import RamifyCoq.veric_ext.SeparationLogic.
 Require Import RamifyCoq.floyd_ext.DataatSL.
+Require Import RamifyCoq.Coqlib.
 
 Local Open Scope logic.
 
-Instance SGS_VST: SpatialGraphSetting.
-  apply (Build_SpatialGraphSetting pointer_val NullPointer PV_eq_dec).
+Instance PointerVal_EqDec: EquivDec.EqDec pointer_val eq.
+  hnf; intros.
+  apply PV_eq_dec.
 Defined.
 
-Definition trinode (sh: share) (p: Addr) (dlr: Val): mpred :=
+Instance PointerValLR_EqDec: EquivDec.EqDec (pointer_val * LR) eq.
+  hnf; intros.
+  destruct x, y.
+  destruct l, l0; [| right | right |]; simpl; try congruence.
+  + destruct (PV_eq_dec p p0); [left | right]; congruence.
+  + destruct (PV_eq_dec p p0); [left | right]; congruence.
+Defined.
+
+Instance SGA_VST: SpatialGraphAssum pointer_val (pointer_val * LR) mpred.
+  refine (Build_SpatialGraphAssum pointer_val (pointer_val * LR) mpred _ _ _ _ _ _).
+Defined.
+
+Instance BMGS_VST: BasicMarkProgramSetting.
+  refine (Build_BasicMarkProgramSetting pointer_val NullPointer mpred _).
+Defined.
+
+Definition trinode (sh: share) (p: addr) (dlr: bool * addr * addr): mpred :=
   match dlr with
   | (d, l, r) => data_at sh node_type
                   (Vint (Int.repr (if d then 1 else 0)), (pointer_val_val l, pointer_val_val r))
                     (pointer_val_val p)
   end.
 
-Instance MSLstandard sh : MapstoSepLog AV_SGraph (trinode sh).
+Instance SGP_VST (sh: share) : SpatialGraphPred addr (addr * LR) (bool * addr * addr) unit pred.
+  refine (Build_SpatialGraphPred _ _ _ _ _ (trinode sh) (fun _ _ => emp)).
+Defined.
+
+Instance MGS_VST (sh: share): MarkProgramSetting.
+  refine (Build_MarkProgramSetting BMGS_VST (SGP_VST sh)).
+Defined.
+
+Instance MSLstandard sh : MapstoSepLog (AAV _ _ _ (addr * LR) _) (trinode sh).
 Proof.
   intros.
   apply mkMapstoSepLog.
@@ -33,11 +60,11 @@ Proof.
   apply data_at_memory_block.
 Defined.
 
-Instance sMSLstandard sh : StaticMapstoSepLog AV_SGraph (trinode sh).
+Instance sMSLstandard sh : StaticMapstoSepLog (AAV _ _ _ (addr * LR) _) (trinode sh).
 Proof.
   apply mkStaticMapstoSepLog; simpl; intros.
-  + hnf in H. simpl in H. unfold addr_eqb in H. simpl in H.
-    destruct PV_eq_dec; congruence.
+  + hnf in H. simpl in H.
+    destruct_eq_dec p p; congruence.
   + unfold trinode.
     destruct v1 as [[d1 l1] r1].
     destruct v2 as [[d2 l2] r2].
@@ -46,8 +73,7 @@ Proof.
     normalize.
     apply data_at_conflict.
     change (sizeof cenv_cs node_type) with 16.
-    unfold addr_eqb in H; simpl in H.
-    destruct (PV_eq_dec p1 p2); [| congruence].
+    destruct_eq_dec p1 p2; [| congruence].
     subst.
     apply pointer_range_overlap_refl; try omega.
     destruct H0; auto.
@@ -69,8 +95,7 @@ Proof.
       apply disj_prop_andp_right; [apply field_compatible_dec | intro].
       apply disj_data_at.
       change (sizeof cenv_cs node_type) with 16.
-      unfold addr_eqb in H; simpl in H.
-      destruct (PV_eq_dec p1 p2); [congruence |].
+      destruct_eq_dec p1 p2; [congruence |].
       destruct H0 as [? [_ [_ [_ [_ [_ [? _]]]]]]].
       destruct H1 as [? [_ [_ [_ [_ [_ [? _]]]]]]].
       unfold align_compatible in *.
@@ -80,15 +105,11 @@ Proof.
       cbv beta iota zeta delta [pointer_val_val] in *; clear H0 H1.
       intros [[? ?] [[? ?] [? [? ?]]]].
       inv H0; inv H1.
-      apply res_predicates.range_overlap_spec in H4; [| omega | omega].
-      assert (Int.unsigned i = Int.unsigned i0) by (destruct H4 as [[? ?] | [? ?]], H3, H2; omega).
-      assert (b = b0) by (destruct H4 as [[? ?] | [? ?]]; subst; auto).
-      apply n.
+      apply res_predicates.range_overlap_spec in H5; [| omega | omega].
+      assert (Int.unsigned i = Int.unsigned i0) by (destruct H5 as [[? ?] | [? ?]], H4, H3; omega).
+      assert (b = b0) by (destruct H5 as [[? ?] | [? ?]]; subst; auto).
+      apply H2.
       rewrite H1, <- (Int.repr_unsigned i), H0, Int.repr_unsigned; auto.
-Defined.
-
-Instance SGA_VST (sh: Share.t) : SpatialGraphAssum.
-  apply (Build_SpatialGraphAssum mpred _ _ _ _ _ _ _ _ SGS_VST (trinode sh) _ (sMSLstandard sh)).
 Defined.
 
 
